cub now separates in and out arguments (#434)
started cub arg refactor

rebasing changes from main

rebasing shift and lifting updates

rebasing removing infer member types

refactoring

updating shift and lift changes

working on new copy in copy out

rebasing with lifting updates

new copyin copyout in big step

editing big step properties proofs

rebasing shifting and lifting updates

editing lemmas

rebasing for set header validity

rebasing for shifting lifting updates

inn out map lemmas

rebasing shifting lifting changes

attempting to prove table case in shift eval

edited lifted proofs

edits

proved one shift stm lemma

another shifting proof for stms

statement shifting lemmas proven

started refactoring interpreter

interpreter refactored

fixed to p4cub

gcl builds

builds

lib/p4cubSexp.ml
@@ -213,15 +213,15 @@ let sexp_of_call = function
       sexp_of_method extern_name name type_args ret
   | Call.Inst (name, ext_args) -> sexp_of_apply name ext_args
 
-let sexp_of_paramarg f = function
-  | PAIn a -> make_sexp "PAIn" [ f a ]
-  | PAOut a -> make_sexp "PAOut" [ f a ]
-  | PAInOut a -> make_sexp "PAInOut" [ f a ]
+let sexp_of_inout f g ({ inn; out } : ('a, 'b) InOut.t) =
+  Sexp.List
+    [
+      Sexp.List [ Sexp.Atom "inn"; f inn ];
+      Sexp.List [ Sexp.Atom "out"; g out ];
+    ]
 
-let sexp_of_param = sexp_of_paramarg sexp_of_type
-let sexp_of_params = sexp_of_dict sexp_of_param
-let sexp_of_arg = sexp_of_paramarg sexp_of_exp
-let sexp_of_args = sexp_of_list sexp_of_arg
+let sexp_of_params = sexp_of_inout (sexp_of_dict sexp_of_type) (sexp_of_dict sexp_of_type)
+let sexp_of_args = sexp_of_inout (sexp_of_list sexp_of_exp) (sexp_of_list sexp_of_exp)
 
 let sexp_of_app call args =
   make_sexp "Stm.App" [ sexp_of_call call; sexp_of_args args ]
@@ -311,9 +311,9 @@ let sexp_of_constructor_param_type = function
 
 let sexp_of_constructor_params = sexp_of_dict sexp_of_constructor_param_type
 
-let sexp_of_function_type ({ paramargs; rtrns } : Typ.arrowT) =
-  let params_sexp = sexp_of_params paramargs in
-  let rtrns_sexp = sexp_of_option sexp_of_type rtrns in
+let sexp_of_function_type ({ inout; ret } : Typ.arrow) =
+  let params_sexp = sexp_of_params inout in
+  let rtrns_sexp = sexp_of_option sexp_of_type ret in
   Sexp.List
     [
       Sexp.List [ Sexp.Atom "paramargs"; params_sexp ];
