coq/lib/GCL/V1model.v
@@ -42,8 +42,8 @@ Definition det_fwd_asst   :=
              (E.Var (Typ.Bit 9%N) "standard_metadata.egress_spec" 0)
              (E.Bit 9%N 0%Z)
   in
-  let paramargs := [(*check*) PAIn assertion] in
-  ST.App (Call.Method "_" "assert" [] None) paramargs.
+  let args := InOut.mk_t [(*check*) assertion] [] in
+  ST.App (Call.Method "_" "assert" [] None) args.
 
 Definition standard_metadata_t : Typ.t :=
   Typ.Struct
@@ -66,38 +66,55 @@ Definition standard_metadata_t : Typ.t :=
      Typ.Bit 3 (*priority*)].
 
 (* TODO: correct de bruijn index? *)
-Definition t_arg (dir : E.t -> paramarg E.t E.t) typ var :=
-  (var, dir (E.Var typ var 0)).
+Definition t_arg typ var :=
+  (var, E.Var typ var 0).
 
 Definition pipeline  (htype mtype : Typ.t) (parser v_check ingress egress c_check deparser : string) : ST.t * ST.t  :=
   let ext_args := ["packet_in"] in
-  let pargs := [
-        t_arg PAOut      htype                "parsedHdr";
-        t_arg PAInOut    mtype                "meta";
-        t_arg PAInOut standard_metadata_t "standard_metadata"] in
-  let vck_args := [
-        t_arg PAInOut htype "hdr";
-        t_arg PAInOut mtype "meta"] in
-  let ing_args := [
-        t_arg PAInOut htype "hdr";
-        t_arg PAInOut mtype "meta";
-        t_arg PAInOut standard_metadata_t "standard_metadata"] in
-  let egr_args := [
-        t_arg PAInOut htype "hdr";
-        t_arg PAInOut mtype "meta";
-        t_arg PAInOut standard_metadata_t "standard_metadata"] in
-  let cck_args := [
-        t_arg PAInOut htype "hdr";
-        t_arg PAInOut mtype "meta"] in
+  let pargs :=
+    InOut.mk_t
+      [t_arg mtype               "meta";
+       t_arg standard_metadata_t "standard_metadata"]
+      [t_arg htype               "parsedHdr";
+       t_arg mtype               "meta";
+       t_arg standard_metadata_t "standard_metadata"] in
+  let vck_args :=
+    InOut.mk_t
+      [t_arg htype "hdr";
+       t_arg mtype "meta"]
+      [t_arg htype "hdr";
+       t_arg mtype "meta"] in
+  let ing_args :=
+    InOut.mk_t
+      [t_arg htype "hdr";
+       t_arg mtype "meta";
+       t_arg standard_metadata_t "standard_metadata"]
+      [t_arg htype "hdr";
+       t_arg mtype "meta";
+       t_arg standard_metadata_t "standard_metadata"] in
+  let egr_args :=
+    InOut.mk_t
+      [t_arg htype "hdr";
+       t_arg mtype "meta";
+       t_arg standard_metadata_t "standard_metadata"]
+      [t_arg htype "hdr";
+       t_arg mtype "meta";
+       t_arg standard_metadata_t "standard_metadata"] in
+  let cck_args :=
+    InOut.mk_t
+      [t_arg htype "hdr";
+       t_arg mtype "meta"]
+      [t_arg htype "hdr";
+       t_arg mtype "meta"] in
   let dep_ext_args := [ "packet_out" ; "b" ] in
-  let dep_args := [ t_arg PAIn htype "hdr"] in
-  (ST.App (Call.Inst parser ext_args) (map snd pargs),
+  (*let dep_args := InOut.mk_t [ t_arg htype "hdr"] [] in*)
+  (ST.App (Call.Inst parser ext_args) (InOut.map_uni snd pargs),
     (* ST.Apply v_check ext_args vck_args i; *)
     ST.Cond
         (E.Var Typ.Bool ("_state$accept$next") 0)
         (cub_seq [
-                 ST.App (Call.Inst ingress ext_args) (map snd ing_args)
-                 ; ST.App (Call.Inst egress ext_args) (map snd egr_args)
+                 ST.App (Call.Inst ingress ext_args) (InOut.map_uni snd ing_args)
+                 ; ST.App (Call.Inst egress ext_args) (InOut.map_uni snd egr_args)
                  (* ; det_fwd_asst *)
         ])
         ST.Skip
@@ -125,7 +142,7 @@ Definition package (types : list Typ.t) (cargs : Top.constructor_args) : result 
 (*   let assume_decl := TopDecl.Extern "_" 1 [] [] [("assume", (0%nat, [], arrowtype))] in *)
 
 Definition gcl_from_p4cub instr hv gas unroll p4cub : result string (ToGCL.target * ToGCL.target) :=
-  let arrowtype := ({|paramargs:=[("check", PAIn Typ.Bool)]; rtrns:=None|} : Typ.arrowT) in
+  let arrowtype := ({|Arr.inout:=InOut.mk_t [("check", Typ.Bool)] []; Arr.ret:=None|} : Typ.arrow) in
   let assume_decl := Top.Extern "_" 1 [] [] [("assume", (0%nat, [], arrowtype))] in
   let p4cub_instrumented := ToP4cub.add_extern  p4cub assume_decl in
   ToGCL.from_p4cub instr hv gas unroll externs (package) p4cub.
