coq/lib/P4cub/Semantics/Dynamic/BigStep/InstUtil.v
@@ -1,20 +1,30 @@
 From Poulet4.P4cub Require Import
   Syntax.AST Semantics.Climate Semantics.Dynamic.BigStep.Value.Syntax.
-Import String Clmt.Notations.
-  
+From RecordUpdate Require Import RecordSet.
+Import String Clmt.Notations RecordSetNotations.
+
+Module Table.
+  Record t : Set :=
+    mk_t
+      { scope : nat (** number of variables in scope. Tables have dynamic scope. *);
+        key : list (Exp.t * string);
+        actions : list (string * Exp.args);
+        default : option (string * list Exp.t)
+      }.
+
+  Global Instance eta_t : Settable _ :=
+    settable! mk_t <scope; key; actions; default>.
+End Table.
+
 (** Table environment. *)
-Definition tenv : Set :=
-  Clmt.t
-    string (** table name. *)
-    (nat (** number of variables in scope. Tables have dynamic scope. *)
-     * list (Exp.t * string) (** table key. *)
-     * list (string * Exp.args) (** actions. *)
-     * option (string * list Exp.t)) (** default action. *).
+Definition table_env : Set :=
+  Clmt.t string (** table name. *) Table.t.
 
 (** Function declarations and closures. *)
 Inductive fdecl: Set :=
 | FDecl (fs : Clmt.t string fdecl) (** function closure *)
-        (body : Stm.t) (** function body *).
+        (params : Typ.params)
+        (body : Stm.t).
 
 (** Function names to closures. *)
 Definition fenv: Set := Clmt.t string fdecl.
@@ -24,7 +34,9 @@ Inductive adecl: Set :=
 | ADecl
     (clos : list Val.t) (** value closure *)
     (actions : Clmt.t string adecl) (** action closure *)
-    (body : Stm.t) (** action body *).
+    (ctrl_params : list Typ.t) (** control-plane parameters *)
+    (data_params : Typ.params) (** data-plane parameters *)
+    (body : Stm.t).
 
 (** Action names to closures. *)
 Definition aenv: Set := Clmt.t string adecl.
@@ -37,21 +49,23 @@ Section Inst.
   | ControlInst
       (fs : fenv) (** function closure *)
       (insts : Clmt.t string inst) (** instance closure *)
-      (tbls : tenv) (** table closure *)
+      (tbls : table_env) (** table closure *)
       (actions : aenv) (** action closure *)
-      (epsilon : list V) (** constructor args *)
+      (vs : list V) (** constructor args *)
+      (params : Typ.params)
       (apply_blk : Stm.t)  (** control instance apply block *)
   | ParserInst
       (fs : fenv) (** function closure *)
       (insts : Clmt.t string inst) (** instance closure *)
-      (epsilon : list V) (** constructor args *)
+      (vs : list V) (** constructor args *)
+      (params : Typ.params)
       (strt : Stm.t) (** start state *)
       (states : list Stm.t) (** other states *)
   | ExternInst
       (fs : fenv) (** function closure *)
       (insts : Clmt.t string inst) (** instance closure *)
-      (epsilon : list V) (** constructor args *)
-  (* TODO: what else? *).
+      (vs : list V) (** constructor args *).
+  (* TODO: what else? *)
   
   Definition inst_env: Set := Clmt.t string inst.
 
@@ -75,19 +89,20 @@ Section Inst.
       (fs : fenv) (** function closure *)
       (insts : inst_env) (** control instance closure *)
       (cparams : list string) (** constructor param names *)
+      (params : Typ.params)
       (body : list Ctrl.t) (** declarations inside control *)
       (apply_block : Stm.t) (** apply block *)
   | ParserDecl
       (fs : fenv) (** function closure *)
       (insts : inst_env) (** parser instance closure *)
       (cparams : list string) (** constructor param names *)
+      (params : Typ.params)
       (strt : Stm.t) (** start state *)
       (states : list Stm.t) (** parser states *)
   | ExternDecl
       (fs : fenv) (** function closure *)
       (insts : Clmt.t string inst) (** instance closure *)
-      (cparams : list string) (** constructor param names *)
-  (** function closure *).
+      (cparams : list string) (** constructor param names *).
 
   Definition top_env: Set := Clmt.t string top_closure.
 End Inst.
